WIP * create a bind notation with yield * try to restore lemmas for opening and closing invariants under wsats

examples/scheduler/SchGInv.v
@@ -13,46 +13,40 @@ End GINV.
 
 Section AUX.
 
-  Context `{!sinvG Σ Γ α β τ}.
+  Context `{@sinvG Σ Γ α β τ}.
   Notation iProp := (iProp Σ).
 
-  (* Global Instance inv_persistent 
-  u n i p : Persistent (inv u n i p).
-  Proof.
-    Local Transparent inv.
-    unfold inv. unfold Persistent. iIntros "#I". iModIntro. iApply "I".
-  Qed. *)
-
-  (* Definition close_inv (u: positive) (n invn: nat) (ns: namespace) (p: SRFSyn.t invn) : iProp :=
-    (⟦p⟧ -∗ closed_universe u n (⊤ ∖ ↑ns) ==∗ closed_universe u n ⊤)%SRF.
+  Definition close_inv (u: positive) (n invn: nat) (ns: namespace) (p: SRFSyn.t invn) : iProp :=
+    (⟦p⟧ -∗ wsats u n (⊤ ∖ ↑ns) ==∗ wsats u n ⊤).
 
   Lemma open_invariant u lv0 lv1 ns p
     (LT: lv0 < lv1)
   :
-    inv u lv0 ns p ∗ closed_universe u lv1 ⊤
-    -∗ ( |==> ⟦ p ⟧ ∗ closed_universe u lv1 (⊤ ∖↑ns) ∗ close_inv u lv1 ns p).
+    inv u lv0 ns p -∗ ( =|u, lv1|={⊤}=> ⟦ p ⟧ ∗ @close_inv u lv1 lv0 ns p).
   Proof.
-    Local Transparent invariants.FUpd.
-    iIntros "[#INV W]".
-    iPoseProof (FUpd_open with "[INV]") as "F"; et.
+    (* iIntros "#INV". ss. iModIntro.
+    iApply elim_acc_fupd.
+    iInv "INV" as "T".
+    Search fupd.
+    iPoseProof (fupd_open with "[INV]") as "F"; et.
     unfold invariants.FUpd. iPoseProof ("F" with "[W]") as "FU".
     { iDestruct "W" as "[U FW]". iFrame. iApply "FW". }
     iMod "FU". iDestruct "FU" as "(FW & W & P & FU)". iFrame.
     iModIntro. iIntros "P CW". iPoseProof ("FU" with "[P]") as "P"; et.
     iPoseProof ("P" with "[CW]") as ">[U [FW _]]".
     { iDestruct "CW" as "[U FW]". iFrame. }
-    iModIntro. iFrame.
-  Qed.
+    iModIntro. iFrame. *)
+  Admitted.
 
   Lemma close_invariant u lv0 lv1 ns p
     (LT: lv0 < lv1)
   :
-    ⟦ p ⟧ ∗ closed_universe u lv1 (⊤∖↑ns) ∗ @close_inv u lv1 lv0 ns p
-    -∗ ( |==> closed_universe u lv1 ⊤).
+    ⟦ p ⟧ ∗ wsats u lv1 (⊤∖↑ns) ∗ @close_inv u lv1 lv0 ns p
+    -∗ ( |==> wsats u lv1 ⊤).
   Proof.
     iIntros "(INV & W & CLOSE)".
     unfold close_inv. iPoseProof ("CLOSE" with "[INV]") as "INV"; et.
     iPoseProof ("INV" with "[W]") as "W"; et.
-  Qed. *)
+  Qed.
     
 End AUX.
